

Task 4 Divide and Conquer Analysis

$$\text{when } T(n) = aT\left(\frac{n}{b}\right) + f(n)$$

$$\text{and R1: } T(n) = 16T\left(\frac{n}{4}\right) + n$$

$$\text{Then } a=16 \text{ and } b=4 \text{ and } f(n)=n$$

Comparing with Case 1:

$$\text{if } f(n) = O(n^{\log_b a - \epsilon}) \text{ for some } \epsilon > 0$$

and assuming/testing $\epsilon = 1$ we get:

$$f(n) = O(n^{\log_4 16 - 1}) \Rightarrow f(n) = O(n^{2-1})$$
$$\quad \quad \quad \downarrow$$
$$\quad \quad \quad n^2 \quad \Rightarrow f(n) = O(n)$$

This shows that Case 1 would work. Then:

$$T(n) = \Theta(n^{\log_b a}) = \underline{\underline{\Theta(n^2)}}$$

Task 4 (or maybe should be 5)

with $T(n) = 4T(n/2) + n$

Hypotheses 1:

1. $T(n) \leq c \cdot n^2$ where $c > 0$ [upper bound]

with: $T(n/2) \leq c \cdot (n/2)^2$

Replacing $T(n/2) \Rightarrow T(n) = 4T(n/2) + n$

$$\leq 4 \left(c \left(\frac{n}{2} \right)^2 \right) + n$$

$$\leq 4 \left(c \cdot \frac{n^2}{4} \right) + n$$

$$\stackrel{*c}{\Rightarrow} 4 \left(c \cdot \frac{n^2}{4} \right) = c \cdot n^2$$

$$\stackrel{*4}{\Rightarrow} 4 \left(\frac{cn^2}{4} \right) = cn^2$$

This is false for $\leftarrow T(n) \leq cn^2 + n$

1. Since

$$\underbrace{cn^2 \leq cn^2 + n}_{\text{false}}$$

Task 4 (or 5)

Hypothesis 2:

$$T(n) \geq cn^2 \text{ where } c > 0 \text{ [lower bound]}$$

$$T(n) = 4 \cdot (T(n/2)) + 2$$

and

$$T(n/2) \geq c(n/2)^2$$

$$\Rightarrow T(n) \geq \underbrace{4(c(n/2)^2)}_{cn^2} + n$$

OR simply

$$\underbrace{T(n) \geq cn^2}_{\text{True}}$$

and hypothesis 2 works

Hypothesis 3:

$$T(n) \leq (cn^2 - b \cdot n) \text{ where } c > 0 \text{ and } b > 0$$

and

$$T(n/2) = c(n/2)^2$$

$$\begin{aligned} \Rightarrow T(n) &= 4T(n/2) + n \\ &\leq 4(c(n/2)^2 - b(n/2)) + n \\ &= 4\left(\frac{cn^2}{4} - \frac{bn}{2}\right) + n \\ &= cn^2 - 2bn + n \\ &= cn^2 - (2b-1)n. \end{aligned}$$

$$T(n) \leq cn^2 - (2b-1)n \leq (cn^2 - bn)$$

Since we can ~~can~~ $n=1$ for proofing:

$$c1^2 - (2b-1)1 \leq c1^2 - b1$$

Removing Constant,

$$\Rightarrow -(2b-1) \leq -b$$

$$\Rightarrow 2b-1 \geq b$$

$$\overset{+b}{\Rightarrow} b \geq 1$$

meaning as long as $b \geq 1$

$$T(n) \leq cn^2 - (2b-1)n \leq cn^2 - bn$$

is valid and hypothesis 3 also
works